defined ind_inv in ind_inv.dfy

src/proofs/no_slashable_attestations/supporting_lemmas/ind_inv3.dfy
@@ -29,27 +29,7 @@ module IndInv3
     import opened Att_Ind_Inv_With_Empty_Initial_Attestation_Slashing_DB2
     import opened Common_Proofs
     import opened DVC_Spec_Axioms
-
-    // TODO
-    predicate inv_sent_validity_predicate_only_for_slots_stored_in_att_slashing_db_hist_helper_body(
-        dv: DVState, 
-        hn: BLSPubkey,
-        hn_state: DVCState,
-        s: Slot
-    )
-    {
-                ( hn in dv.consensus_on_attestation_data[s].honest_nodes_validity_functions.Keys
-                    ==> s in hn_state.attestation_consensus_engine_state.att_slashing_db_hist.Keys
-                )
-    }
-
-    predicate inv_sent_validity_predicate_only_for_slots_stored_in_att_slashing_db_hist_helper(dv: DVState)
-    {
-        forall hn: BLSPubkey, s: Slot |
-            hn in dv.honest_nodes_states
-            :: 
-            inv_sent_validity_predicate_only_for_slots_stored_in_att_slashing_db_hist_helper_body(dv, hn, dv.honest_nodes_states[hn], s)        
-    }  
+ 
 
     lemma lemma_att_slashing_db_hist_is_monotonic_f_serve_attestation_duty(
         process: DVCState,
